perf: improve bv_decide performance with large literals (#6453)
This PR improves bv_decide's performance in the presence of large
literals.

The core change of this PR is the reformulation of the reflection code
for literals to:
```diff
 def eval (assign : Assignment) : BVExpr w → BitVec w
   | .var idx =>
-    let ⟨bv⟩ := assign.get idx
-    bv.truncate w
+    let packedBv := assign.get idx
+    /-
+    This formulation improves performance, as in a well formed expression the condition always holds
+    so there is no need for the more involved `BitVec.truncate` logic.
+    -/
+    if h : packedBv.w = w then
+      h ▸ packedBv.bv
+    else
+      packedBv.bv.truncate w
```
The remainder is merely further simplifications that make the terms
smaller and easier to deal with in general. This change is motivated by
applying the following diff to the kernel:
```diff
diff --git a/src/kernel/type_checker.cpp b/src/kernel/type_checker.cpp
index b0e6844dca..f13bb96bd4 100644
--- a/src/kernel/type_checker.cpp
+++ b/src/kernel/type_checker.cpp
@@ -518,6 +518,7 @@ optional<constant_info> type_checker::is_delta(expr const & e) const {
 optional<expr> type_checker::unfold_definition_core(expr const & e) {
     if (is_constant(e)) {
         if (auto d = is_delta(e)) {
+//            std::cout << "Working on unfolding: " << d->get_name() << std::endl;
             if (length(const_levels(e)) == d->get_num_lparams()) {
                 if (m_diag) {
                     m_diag->record_unfold(d->get_name());
```
and observing that in the test case from #6043 we see a long series of
```
Working on unfolding: Bool.decEq
Working on unfolding: Bool.decEq.match_1
Working on unfolding: Bool.casesOn
Working on unfolding: Nat.ble
Working on unfolding: Nat.brecOn
Working on unfolding: Nat.beq.match_1
Working on unfolding: Nat.casesOn
Working on unfolding: Nat.casesOn
Working on unfolding: Nat.beq.match_1
Working on unfolding: Nat.casesOn
Working on unfolding: Nat.casesOn
```
the chain begins with `BitVec.truncate`, works through a few
abstractions and then continues like above forever, so I avoid the call
to truncate like this. It is not quite clear to me why removing `ofBool`
helps so much here, maybe some other kernel heuristic kicks in to rescue
us.

Either way this diff is a general improvement for reflection of `BitVec`
constants as we should never have to run `BitVec.truncate` again!

Fixes: #6043

src/Std/Tactic/BVDecide/Bitblast/BVExpr/Basic.lean
@@ -293,8 +293,15 @@ The semantics for `BVExpr`.
 -/
 def eval (assign : Assignment) : BVExpr w → BitVec w
   | .var idx =>
-    let ⟨bv⟩ := assign.get idx
-    bv.truncate w
+    let packedBv := assign.get idx
+    /-
+    This formulation improves performance, as in a well formed expression the condition always holds
+    so there is no need for the more involved `BitVec.truncate` logic.
+    -/
+    if h : packedBv.w = w then
+      h ▸ packedBv.bv
+    else
+      packedBv.bv.truncate w
   | .const val => val
   | .zeroExtend v expr => BitVec.zeroExtend v (eval assign expr)
   | .extract start len expr => BitVec.extractLsb' start len (eval assign expr)
@@ -308,8 +315,13 @@ def eval (assign : Assignment) : BVExpr w → BitVec w
   | .arithShiftRight lhs rhs => BitVec.sshiftRight' (eval assign lhs) (eval assign rhs)
 
 @[simp]
-theorem eval_var : eval assign ((.var idx) : BVExpr w) = (assign.get idx).bv.truncate _ := by
-  rfl
+theorem eval_var : eval assign ((.var idx) : BVExpr w) = (assign.get idx).bv.truncate w := by
+  rw [eval]
+  split
+  · next h =>
+    subst h
+    simp
+  · rfl
 
 @[simp]
 theorem eval_const : eval assign (.const val) = val := by rfl
@@ -454,7 +466,7 @@ def eval (assign : BVExpr.Assignment) (expr : BVLogicalExpr) : Bool :=
 @[simp] theorem eval_not : eval assign (.not x) = !eval assign x := rfl
 @[simp] theorem eval_gate : eval assign (.gate g x y) = g.eval (eval assign x) (eval assign y) := rfl
 @[simp] theorem eval_ite :
-  eval assign (.ite d l r) = if (eval assign d) then (eval assign l) else (eval assign r) := rfl
+  eval assign (.ite d l r) = bif (eval assign d) then (eval assign l) else (eval assign r) := rfl
 
 def Sat (x : BVLogicalExpr) (assign : BVExpr.Assignment) : Prop := eval assign x = true
 
