src/Std/Tactic/BVDecide/Normalize/Bool.lean
@@ -41,7 +41,14 @@ attribute [bv_normalize] Bool.not_not
 attribute [bv_normalize] Bool.and_self_left
 attribute [bv_normalize] Bool.and_self_right
 attribute [bv_normalize] eq_self
-attribute [bv_normalize] ite_self
+attribute [bv_normalize] Bool.cond_self
+attribute [bv_normalize] cond_false
+attribute [bv_normalize] cond_true
+attribute [bv_normalize] Bool.cond_not
+
+@[bv_normalize]
+theorem if_eq_cond {b : Bool} {x y : α} : (if b = true then x else y) = (bif b then x else y) := by
+  rw [cond_eq_if]
 
 @[bv_normalize]
 theorem Bool.not_xor : ∀ (a b : Bool), !(a ^^ b) = (a == b) := by decide
